Util.v
@@ -21,7 +21,7 @@ induction l.
     simpl in H. auto.
 Qed.
 
-Lemma in_fst (* unused *){A B : Type} a (l : list (A * B)) :
+Lemma in_fst {A B : Type} a (l : list (A * B)) :
   In a (map fst l)
   -> exists b, In (a,b) l.
 Proof.
